changing definition of OrLinv1/2

ljt/ljt_inv.v
@@ -27,11 +27,11 @@ Inductive ImpLinv2 {V} : relationT (list (PropF V)) :=
 (*
 Inductive AndLinv {V} : relationT (list (PropF V)) :=
   | AndLinv_I : forall C D, AndLinv ([And C D]) ([C ; D]).
-  *)
 Inductive OrLinv1 {V} : relationT (list (PropF V)) :=
   | OrLinv1_I : forall C D, OrLinv1 [Or C D] [C].
 Inductive OrLinv2 {V} : relationT (list (PropF V)) :=
   | OrLinv2_I : forall C D, OrLinv2 [Or C D] [D].
+  *)
 Inductive ImpL_And_inv {V} : relationT (list (PropF V)) :=
   | ImpL_And_inv_I : forall B C D,
     ImpL_And_inv ([Imp (And C D) B]) ([Imp C (Imp D B)]).
@@ -40,16 +40,28 @@ Inductive ImpL_Or_inv1 {V} : relationT (list (PropF V)) :=
 Inductive ImpL_Or_inv2 {V} : relationT (list (PropF V)) :=
   | ImpL_Or_inv2_I : forall B C D, ImpL_Or_inv2 [Imp (Or C D) B] [Imp D B].
 
-Inductive AndLinv1 {V} :  PropF V -> list (PropF V) -> Type :=
-  | AndLinv1_I : forall C D, AndLinv1 (And C D) ([C ; D]).
+Inductive AndLinvs {V} :  PropF V -> list (PropF V) -> Type :=
+  | AndLinvs_I : forall C D, AndLinvs (And C D) ([C ; D]).
+Inductive OrLinv1s {V} : PropF V -> list (PropF V) -> Type :=
+  | OrLinv1s_I : forall C D, OrLinv1s (Or C D) [C].
+Inductive OrLinv2s {V} : PropF V -> list (PropF V) -> Type :=
+  | OrLinv2s_I : forall C D, OrLinv2s (Or C D) [D].
 
 Inductive fslr U W R : list U -> W -> Type := 
   | fslr_I : forall (u : U) (w : W), R u w -> fslr R [u] w. 
 
-Definition AndLinv {V} := fslr (@AndLinv1 V).
+Definition AndLinv {V} := fslr (@AndLinvs V).
+Definition OrLinv1 {V} := fslr (@OrLinv1s V).
+Definition OrLinv2 {V} := fslr (@OrLinv2s V).
 
 Lemma AndLinv_I {V} (C D : PropF V) : AndLinv [And C D] [C; D].
-Proof. apply fslr_I. apply AndLinv1_I. Qed.
+Proof. apply fslr_I. apply AndLinvs_I. Qed.
+
+Lemma OrLinv1_I {V} (C D : PropF V) : OrLinv1 [Or C D] [C].
+Proof. apply fslr_I. apply OrLinv1s_I. Qed.
+
+Lemma OrLinv2_I {V} (C D : PropF V) : OrLinv2 [Or C D] [D].
+Proof. apply fslr_I. apply OrLinv2s_I. Qed.
 
 (* extend relation with general context on the left and a singleton on the 
   right, suitable for ImpLinv2, AndLinv. OrLinv1/2 *)
@@ -95,15 +107,16 @@ Proof. intro ljnc.  eexists. split. apply asmI.
 apply ForallT_singleI.  eexists. split.  2: apply rT_refl.
 apply LJIE in ljnc. subst. simpl. apply InT_cons. apply InT_eq. Qed.
 
-Lemma lr_And' V Y rules Γ1 Γ2 ps0 C D p 
-  (LJAE : forall ps A B G, rules ps ([And A B], G) -> ps = [([A; B], G)]) :
-  rules ps0 ([@And V C D], p : Y) ->
-  {ps' & derl (fst_ext_rls rules) ps' (Γ1 ++ [C ; D] ++ Γ2, p) *
+Lemma lr_geni U Y rules Γ1 Γ2 ps0 fml fmlsi any p 
+  (LJIE : forall ps G, rules ps ([fml], G) -> InT (fmlsi, G) ps) :
+  rules ps0 ([fml : U], p : Y) ->
+  {ps' & derl (fst_ext_rls rules) ps' (Γ1 ++ fmlsi ++ Γ2, p) *
   ForallT (fun p' => {p0 & InT p0 (map (apfst (fmlsext Γ1 Γ2)) ps0) *
-     clos_reflT (srs_ext_rel AndLinv) p0 p'}) ps'}.
+     clos_reflT (srs_ext_rel any) p0 p'}) ps'}.
 Proof. intro ljnc.  eexists. split. apply asmI.
 apply ForallT_singleI.  eexists. split.  2: apply rT_refl.
-apply LJAE in ljnc. subst. simpl. apply InT_eq. Qed.
+apply LJIE in ljnc. 
+eapply arg1_cong_imp.  2: exact (InT_map _ ljnc).  reflexivity. Qed.
 
 Lemma lr_gen U Y rules Γ1 Γ2 ps0 fml fmlsi any p 
   (LJAE : forall ps G, rules ps ([fml], G) -> ps = [(fmlsi, G)]) :
@@ -111,33 +124,8 @@ Lemma lr_gen U Y rules Γ1 Γ2 ps0 fml fmlsi any p
   {ps' & derl (fst_ext_rls rules) ps' (Γ1 ++ fmlsi ++ Γ2, p) *
   ForallT (fun p' => {p0 & InT p0 (map (apfst (fmlsext Γ1 Γ2)) ps0) *
      clos_reflT (srs_ext_rel any) p0 p'}) ps'}.
-Proof. intro ljnc.  eexists. split. apply asmI.
-apply ForallT_singleI.  eexists. split.  2: apply rT_refl.
-apply LJAE in ljnc. subst. simpl. apply InT_eq. Qed.
-
-Lemma lr_And V Γ1 Γ2 ps0 C D p : @LJncrules V ps0 ([And C D], p) ->
-  {ps' & derl LJrules ps' (Γ1 ++ [C ; D] ++ Γ2, p) *
-  ForallT (fun p' => {p0 & InT p0 (map (apfst (fmlsext Γ1 Γ2)) ps0) *
-     clos_reflT (srs_ext_rel AndLinv) p0 p'}) ps'}.
-Proof. intro ljnc.  eexists. split. apply asmI.
-apply ForallT_singleI.  eexists. split.  2: apply rT_refl.
-apply LJAE in ljnc. subst. simpl. apply InT_eq. Qed.
-
-Lemma lr_Or1 V Γ1 Γ2 ps0 C D p : @LJncrules V ps0 ([Or C D], p) ->
-  {ps' & derl LJrules ps' (Γ1 ++ [C] ++ Γ2, p) *
-  ForallT (fun p' => {p0 & InT p0 (map (apfst (fmlsext Γ1 Γ2)) ps0) *
-     clos_reflT (srs_ext_rel OrLinv1) p0 p'}) ps'}.
-Proof. intro ljnc.  eexists. split. apply asmI.
-apply ForallT_singleI.  eexists. split.  2: apply rT_refl.
-apply LJOE in ljnc. subst. simpl. apply InT_eq. Qed.
-
-Lemma lr_Or2 V Γ1 Γ2 ps0 C D p : @LJncrules V ps0 ([Or C D], p) ->
-  {ps' & derl LJrules ps' (Γ1 ++ [D] ++ Γ2, p) *
-  ForallT (fun p' => {p0 & InT p0 (map (apfst (fmlsext Γ1 Γ2)) ps0) *
-     clos_reflT (srs_ext_rel OrLinv2) p0 p'}) ps'}.
-Proof. intro ljnc.  eexists. split. apply asmI.
-apply ForallT_singleI.  eexists. split.  2: apply rT_refl.
-apply LJOE in ljnc. subst. simpl. apply InT_cons. apply InT_eq. Qed.
+Proof. apply lr_geni. intros * rpg.
+rewrite (LJAE ps G rpg). apply InT_eq. Qed.
 
 Print Implicit lr_Imp2.
 
@@ -265,215 +253,12 @@ Qed.
 
 Print Implicit can_trf_ImpLinv2_lj.
 
-(*
-Lemma can_trf_AndLinv_lj V ps c: @LJrules _ ps c ->
-  can_trf_rules_rc (srs_ext_rel (@AndLinv V)) (derl (@LJrules _)) ps c.
-Proof. intro ljpc. destruct ljpc. inversion r. subst. clear r.
-unfold can_trf_rules_rc. intros c' ser.
-inversion ser. clear ser. destruct c0. simpl in H.
-unfold fmlsext in H. inversion H. clear H. subst.
-destruct H0.  (* pose (LJnc_seL X). *)
-acacD'T2 ; subst.
-- rewrite ?app_nil_r in X. 
-assoc_mid H3.  eexists. split.  apply ncdlj. apply X.
-apply fcr. intro. destruct q. 
-apserx. apply AndLinv_I.
-- pose (LJnc_seL X).  apply sing_empty_app_cons in s.
-list_eq_ncT. cD. subst. simpl.  simpl in X. rewrite ?app_nil_r.
-apply (lr_And _ _ X).
-- pose (LJnc_seL X).  apply sing_empty_app_cons in s.
-cD. subst. simpl.  simpl in X. rewrite ?app_nil_r.
-apply (lr_And _ _ X).
-- eexists. split. assoc_mid l. apply ncdlj. apply X.
-apply fcr. intro. destruct q. 
-apserx. apply AndLinv_I.
-- pose (LJnc_seL X).
-apply sing_empty_app in s. sD. inversion s. subst. simpl.
-rewrite ?app_nil_r in X.  rewrite ?app_nil_r.
-apply (lr_And _ _ X).
-- list_eq_ncT. cD. subst. simpl in X.
-eexists. split. assoc_mid H4. apply ncdlj. apply X.
-apply fcr. intro. destruct q. 
-apserx. apply AndLinv_I.
-- list_eq_ncT. sD ; subst.
-+ eexists. split.  apply ncdlje. apply X.
-apply fcr. intro. destruct q. 
-rewrite ?app_nil_r.
-apserx. apply AndLinv_I.
-+ simpl. rewrite ?app_nil_r.  apply (lr_And _ _ X).
-- list_eq_ncT. cD.  list_eq_ncT. cD. subst. (* simpl. NO! *) list_assoc_l'.
-eexists. split. apply ncdlje. apply X.
-apply fcr. intro. destruct q. 
-apserx. apply AndLinv_I.
-- eexists. split. assoc_mid l. apply ncdlj. apply X.
-apply fcr. intro. destruct q. 
-list_assoc_r'. simpl.  
-apserx. apply AndLinv_I.
-Qed.
-
-Print Implicit can_trf_AndLinv_lj.
-*)
-
-Lemma can_trf_OrLinv1_lj V ps c: @LJrules _ ps c ->
-  can_trf_rules_rc (srs_ext_rel (@OrLinv1 V)) (derl (@LJrules _)) ps c.
-Proof. intro ljpc. destruct ljpc. inversion r. subst. clear r.
-unfold can_trf_rules_rc. intros c' ser.
-inversion ser. clear ser. destruct c0. simpl in H.
-unfold fmlsext in H. inversion H. clear H. subst.
-destruct H0.  (* pose (LJnc_seL X). *)
-acacD'T2 ; subst.
-- rewrite ?app_nil_r in X. 
-assoc_mid H3.  eexists. split.  apply ncdlj. apply X.
-apply fcr. intro. destruct q. 
-apserx. apply OrLinv1_I.
-- pose (LJnc_seL X).  apply sing_empty_app_cons in s.
-list_eq_ncT. cD. subst. simpl.  simpl in X. rewrite ?app_nil_r.
-apply (lr_Or1 _ _ X).
-- pose (LJnc_seL X).  apply sing_empty_app_cons in s.
-cD. subst. simpl.  simpl in X. rewrite ?app_nil_r.
-apply (lr_Or1 _ _ X).
-- eexists. split. assoc_mid l. apply ncdlj. apply X.
-apply fcr. intro. destruct q. 
-apserx. apply OrLinv1_I.
-- pose (LJnc_seL X).
-apply sing_empty_app in s. sD. inversion s. subst. simpl.
-rewrite ?app_nil_r in X.  rewrite ?app_nil_r.
-apply (lr_Or1 _ _ X).
-- list_eq_ncT. cD. subst. simpl in X.
-eexists. split. assoc_mid H4. apply ncdlj. apply X.
-apply fcr. intro. destruct q. 
-apserx. apply OrLinv1_I.
-- list_eq_ncT. sD ; subst.
-+ eexists. split.  apply ncdlje. apply X.
-apply fcr. intro. destruct q. 
-rewrite ?app_nil_r.
-apserx. apply OrLinv1_I.
-+ simpl. rewrite ?app_nil_r.  apply (lr_Or1 _ _ X).
-- list_eq_ncT. cD.  list_eq_ncT. cD. subst. (* simpl. NO! *) list_assoc_l'.
-eexists. split. apply ncdlje. apply X.
-apply fcr. intro. destruct q. 
-apserx. apply OrLinv1_I.
-- eexists. split. assoc_mid l. apply ncdlj. apply X.
-apply fcr. intro. destruct q. 
-list_assoc_r'. simpl.  
-apserx. apply OrLinv1_I.
-Qed.
-
-Print Implicit can_trf_OrLinv1_lj.
-
-Lemma can_trf_OrLinv2_lj V ps c: @LJrules _ ps c ->
-  can_trf_rules_rc (srs_ext_rel (@OrLinv2 V)) (derl (@LJrules _)) ps c.
-Proof. intro ljpc. destruct ljpc. inversion r. subst. clear r.
-unfold can_trf_rules_rc. intros c' ser.
-inversion ser. clear ser. destruct c0. simpl in H.
-unfold fmlsext in H. inversion H. clear H. subst.
-destruct H0.  (* pose (LJnc_seL X). *)
-acacD'T2 ; subst.
-- rewrite ?app_nil_r in X. 
-assoc_mid H3.  eexists. split.  apply ncdlj. apply X.
-apply fcr. intro. destruct q. 
-apserx. apply OrLinv2_I.
-- pose (LJnc_seL X).  apply sing_empty_app_cons in s.
-list_eq_ncT. cD. subst. simpl.  simpl in X. rewrite ?app_nil_r.
-apply (lr_Or2 _ _ X).
-- pose (LJnc_seL X).  apply sing_empty_app_cons in s.
-cD. subst. simpl.  simpl in X. rewrite ?app_nil_r.
-apply (lr_Or2 _ _ X).
-- eexists. split. assoc_mid l. apply ncdlj. apply X.
-apply fcr. intro. destruct q. 
-apserx. apply OrLinv2_I.
-- pose (LJnc_seL X).
-apply sing_empty_app in s. sD. inversion s. subst. simpl.
-rewrite ?app_nil_r in X.  rewrite ?app_nil_r.
-apply (lr_Or2 _ _ X).
-- list_eq_ncT. cD. subst. simpl in X.
-eexists. split. assoc_mid H4. apply ncdlj. apply X.
-apply fcr. intro. destruct q. 
-apserx. apply OrLinv2_I.
-- list_eq_ncT. sD ; subst.
-+ eexists. split.  apply ncdlje. apply X.
-apply fcr. intro. destruct q. 
-rewrite ?app_nil_r.
-apserx. apply OrLinv2_I.
-+ simpl. rewrite ?app_nil_r.  apply (lr_Or2 _ _ X).
-- list_eq_ncT. cD.  list_eq_ncT. cD. subst. (* simpl. NO! *) list_assoc_l'.
-eexists. split. apply ncdlje. apply X.
-apply fcr. intro. destruct q. 
-apserx. apply OrLinv2_I.
-- eexists. split. assoc_mid l. apply ncdlj. apply X.
-apply fcr. intro. destruct q. 
-list_assoc_r'. simpl.  
-apserx. apply OrLinv2_I.
-Qed.
-
-Print Implicit can_trf_OrLinv2_lj.
 Print Implicit der_trf_rc_derl.
 
-(* try to redo the above, more generally *)
-(*
-Lemma can_trf_AndLinv_gen V Y rules ps c
-  (nc_seL : forall ps cl cr, rules ps (cl, cr) -> sing_empty cl) 
-  (LJAE : forall ps A B G, rules ps ([And A B], G) -> ps = [([A; B], G)]) :
-  fst_ext_rls rules ps c ->
-  can_trf_rules_rc (@srs_ext_rel _ Y (@AndLinv V)) 
-    (derl (fst_ext_rls rules)) ps c.
-Proof. intro ljpc. destruct ljpc. inversion r. subst. clear r.
-unfold can_trf_rules_rc. intros c' ser.
-inversion ser. clear ser. destruct c0. simpl in H.
-unfold fmlsext in H. inversion H. clear H. subst.
-destruct H0.  (* pose (LJnc_seL X). *)
-acacD'T2 ; subst.
-- rewrite ?app_nil_r in X. 
-assoc_mid H3.  eexists. split.  apply ncdgen. apply X.
-apply fcr. intro. destruct q. 
-apserx. apply AndLinv_I.
-- pose (nc_seL _ _ _ X).  apply sing_empty_app_cons in s.
-list_eq_ncT. cD. subst. simpl.  simpl in X. rewrite ?app_nil_r.
-apply lr_And'. exact LJAE. exact X.
-- pose (nc_seL _ _ _ X).  apply sing_empty_app_cons in s.
-cD. subst. simpl.  simpl in X. rewrite ?app_nil_r.
-apply lr_And'. exact LJAE. exact X.
-- eexists. split. assoc_mid l. apply ncdgen. apply X.
-apply fcr. intro. destruct q. 
-apserx. apply AndLinv_I.
-- pose (nc_seL _ _ _ X).
-apply sing_empty_app in s. sD. inversion s. subst. simpl.
-rewrite ?app_nil_r in X.  rewrite ?app_nil_r.
-apply lr_And'. exact LJAE. exact X.
-- list_eq_ncT. cD. subst. simpl in X.
-eexists. split. assoc_mid H4. apply ncdgen. apply X.
-apply fcr. intro. destruct q. 
-apserx. apply AndLinv_I.
-- list_eq_ncT. sD ; subst.
-+ eexists. split.  apply ncdgene. apply X.
-apply fcr. intro. destruct q. 
-rewrite ?app_nil_r.
-apserx. apply AndLinv_I.
-+ simpl. rewrite ?app_nil_r.  
-apply lr_And'. exact LJAE. exact X.
-- list_eq_ncT. cD.  list_eq_ncT. cD. subst. (* simpl. NO! *) list_assoc_l'.
-eexists. split. apply ncdgene. apply X.
-apply fcr. intro. destruct q. 
-apserx. apply AndLinv_I.
-- eexists. split. assoc_mid l. apply ncdgen. apply X.
-apply fcr. intro. destruct q. 
-list_assoc_r'. simpl.  
-apserx. apply AndLinv_I.
-Qed.
-
-Print Implicit can_trf_AndLinv_gen.
-
-Print Implicit can_trf_AndLinv_lj.
-
-Lemma can_trf_AndLinv_lj' V ps c: @LJrules _ ps c ->
-  can_trf_rules_rc (srs_ext_rel (@AndLinv V)) (derl (@LJrules _)) ps c.
-Proof. apply can_trf_AndLinv_gen.  apply LJnc_seL.  apply LJAE.  Qed.
-*)
-
-Lemma can_trf_genLinv_gen W Y rules genLinv ps c
+Lemma can_trf_genLinv_geni W Y rules genLinv ps c
   (nc_seL : forall ps cl cr, rules ps (cl, cr) -> sing_empty cl) 
   (rls_unique : forall ps u w G, 
-    genLinv u w -> rules ps ([u], G) -> ps = [(w, G)]) :
+    genLinv u w -> rules ps ([u], G) -> InT (w, G) ps) :
   fst_ext_rls rules ps c ->
   can_trf_rules_rc (@srs_ext_rel W Y (fslr genLinv)) 
     (derl (fst_ext_rls rules)) ps c.
@@ -489,17 +274,17 @@ apply fcr. intro. destruct q.
 apserx. apply fslr_I. exact g.
 - pose (nc_seL _ _ _ X).  apply sing_empty_app_cons in s.
 list_eq_ncT. cD. subst. simpl.  simpl in X. rewrite ?app_nil_r.
-eapply lr_gen. 2: exact X. intros *.  apply rls_unique. exact g.
+eapply lr_geni. 2: exact X. intros *.  apply rls_unique. exact g.
 - pose (nc_seL _ _ _ X).  apply sing_empty_app_cons in s.
 cD. subst. simpl.  simpl in X. rewrite ?app_nil_r.
-eapply lr_gen. 2: exact X. intros *.  apply rls_unique. exact g.
+eapply lr_geni. 2: exact X. intros *.  apply rls_unique. exact g.
 - eexists. split. assoc_mid l. apply ncdgen. apply X.
 apply fcr. intro. destruct q. 
 apserx. apply fslr_I. exact g.
 - pose (nc_seL _ _ _ X).
 apply sing_empty_app in s. sD. inversion s. subst. simpl.
 rewrite ?app_nil_r in X.  rewrite ?app_nil_r.
-eapply lr_gen. 2: exact X. intros *.  apply rls_unique. exact g.
+eapply lr_geni. 2: exact X. intros *.  apply rls_unique. exact g.
 - list_eq_ncT. cD. subst. simpl in X.
 eexists. split. assoc_mid H4. apply ncdgen. apply X.
 apply fcr. intro. destruct q. 
@@ -510,7 +295,7 @@ apply fcr. intro. destruct q.
 rewrite ?app_nil_r.
 apserx. apply fslr_I. exact g.
 + simpl. rewrite ?app_nil_r.  
-eapply lr_gen. 2: exact X. intros *.  apply rls_unique. exact g.
+eapply lr_geni. 2: exact X. intros *.  apply rls_unique. exact g.
 - list_eq_ncT. cD.  list_eq_ncT. cD. subst. (* simpl. NO! *) list_assoc_l'.
 eexists. split. apply ncdgene. apply X.
 apply fcr. intro. destruct q. 
@@ -520,6 +305,18 @@ apply fcr. intro. destruct q.
 list_assoc_r'. simpl.  
 apserx. apply fslr_I. exact g.
 Qed.
+
+Print Implicit can_trf_genLinv_geni.
+
+Lemma can_trf_genLinv_gen W Y rules genLinv ps c
+  (nc_seL : forall ps cl cr, rules ps (cl, cr) -> sing_empty cl) 
+  (rls_unique : forall ps u w G, 
+    genLinv u w -> rules ps ([u], G) -> ps = [(w, G)]) :
+  fst_ext_rls rules ps c ->
+  can_trf_rules_rc (@srs_ext_rel W Y (fslr genLinv)) 
+    (derl (fst_ext_rls rules)) ps c.
+Proof. apply can_trf_genLinv_geni. exact nc_seL.
+intros * guw rpg. rewrite (rls_unique _ _ _ _ guw rpg). apply InT_eq. Qed.
 
 Print Implicit can_trf_genLinv_gen.
 
@@ -532,25 +329,12 @@ Lemma can_trf_AndLinv_gen' V Y rules ps c
   (nc_seL : forall ps cl cr, rules ps (cl, cr) -> sing_empty cl) 
   (LJAE : forall ps A B G, rules ps ([And A B], G) -> ps = [([A; B], G)]) :
   fst_ext_rls rules ps c ->
-  can_trf_rules_rc (@srs_ext_rel _ Y (fslr (@AndLinv1 V))) 
+  can_trf_rules_rc (@srs_ext_rel _ Y (fslr (@AndLinvs V))) 
     (derl (fst_ext_rls rules)) ps c.
 Proof. eapply can_trf_genLinv_gen.
 exact nc_seL. intros * auw. destruct auw. apply LJAE. Qed.
 
 Check can_trf_rules_rc_rel_eqv.
-
-(*
-Lemma can_trf_AndLinv_gen'' V Y rules ps c
-  (nc_seL : forall ps cl cr, rules ps (cl, cr) -> sing_empty cl) 
-  (LJAE : forall ps A B G, rules ps ([And A B], G) -> ps = [([A; B], G)]) :
-  fst_ext_rls rules ps c ->
-  can_trf_rules_rc (@srs_ext_rel _ Y (@AndLinv V)) 
-    (derl (fst_ext_rls rules)) ps c.
-Proof. intro frpc.
-eapply can_trf_rules_rc_rel_eqv.
-eapply can_trf_genLinv_gen.
-exact nc_seL. intros * auw. destruct auw. apply LJAE. Qed.
-*)
 
 About can_trf_genLinv_gen.
 
@@ -559,6 +343,18 @@ Lemma can_trf_AndLinv_lj V ps c: @LJrules _ ps c ->
   can_trf_rules_rc (srs_ext_rel (@AndLinv V)) (derl (@LJrules _)) ps c.
 Proof. apply can_trf_genLinv_gen.  apply LJnc_seL.
 intros * auv.  destruct auv.  apply LJAE.  Qed.
+
+Lemma can_trf_OrLinv1_lj V ps c: @LJrules _ ps c ->
+  can_trf_rules_rc (srs_ext_rel (@OrLinv1 V)) (derl (@LJrules _)) ps c.
+Proof. apply can_trf_genLinv_geni.  apply LJnc_seL.
+intros * auv.  destruct auv. intro rocd.  
+apply LJOE in rocd. subst. solve_InT.  Qed.
+
+Lemma can_trf_OrLinv2_lj V ps c: @LJrules _ ps c ->
+  can_trf_rules_rc (srs_ext_rel (@OrLinv2 V)) (derl (@LJrules _)) ps c.
+Proof. apply can_trf_genLinv_geni.  apply LJnc_seL.
+intros * auv.  destruct auv. intro rocd.  
+apply LJOE in rocd. subst. solve_InT.  Qed.
 
 (* now inversion results in terms of rel_adm *)
 Lemma rel_adm_AndLinv V :
@@ -585,4 +381,3 @@ apply der_trf_rc_derl.  exact (@can_trf_ImpLinv2_lj V).  Qed.
 Lemma rel_adm_ImpLinv2 V :
   rel_adm LJrules (srs_ext_rel (@ImpLinv2 V)).
 Proof. apply crd_ra. apply can_rel_ImpLinv2. Qed.
-
